\documentclass{article}
\usepackage{setspace}
\usepackage{amsmath}
\usepackage{amstext}
\usepackage{amssymb}
\usepackage{amsthm}
\usepackage{graphicx} 
\usepackage{float} 
\usepackage{fancyhdr}                                
\usepackage{lastpage}          
\usepackage{textcomp}                               
\usepackage{layout}   
\usepackage{subfigure} 
\pagestyle{fancy}  
\lhead{ZHANG HUAKANG}
\chead{Assignment 7} 
\rhead{DB92760} 
\renewcommand{\baselinestretch}{1.05}
\title{Assignment 7 of MATH 2005}
\author{ZHANG Huakang/DB92760}

\begin{document}
    \maketitle

    \section{}
        \begin{equation*}
            \begin{split}
                G(y)=&F(\sqrt{y})\\
                    =&\int_0 ^{\sqrt{y}} 2se^{-s^2}ds\\
                    =&-e^{-s^2}|_0^{\sqrt{y}}\\
                    =&1-e^{-y}\\
                g(y)=&\frac{d}{dy}G(y)\\
                    =&e^{-y}
            \end{split}
        \end{equation*}
        when $y>0$, and $g(y)=0$ elsewhere.

    \section{}
        \begin{equation*}
            \begin{split}
                G(y)=&F(e^y)\\
                    =&\int _0 ^{e^y} \frac{1}{\theta}e^{-\frac{s}{\theta}}ds\\
                    =&-e^{-\frac{s}{\theta}}|_0^{e^y}\\
                    =&1-e^{-\frac{e^y}{\theta}}\\
                g(y)=&\frac{d}{dy}G(y)\\    
                    =&\frac{1}{\theta}e^{y-\frac{e^y}{\theta}}
            \end{split}
        \end{equation*}
        when $y\in \mathbb{R}$
    \section{}
        \begin{equation*}
            \begin{split}
                G(y)=&F(y^2)\\
                    =&\int _0 ^{y^2} d ds\\
                    =&s|_0^{y^2}\\
                    =&y^2\\
                g(y)=&\frac{d}{dy}y^2\\
                    =&2y\\
            \end{split}
        \end{equation*}
        when $0<y<1$, and $g(y)=0$ elsewhere.

    \section{}
        \paragraph{
            Let $w(y)=\log y$, thus $w'(y)=\frac{1}{y}\neq 0$
            \begin{equation*}
                \begin{split}
                    \varphi(y)=&\varphi(w(y);\mu,\sigma)|w'(y)|\\
                        =&\frac{1}{\sigma\sqrt{2\pi}}e^{-\frac{(\log y-\mu)^2}{2\sigma^2}}\frac{1}{y}
                \end{split}
            \end{equation*}
            when $y\in \mathbb{R}$
        }

    \section{}
        \paragraph{
            We get
            $$f(x)=1$$
            when $0<x<1$
            and $$f(x)=0$$ elsewhere
        }
        \subsection{}
            \paragraph{
                Let $w(y)=e^{-\frac{1}{2}y}$, and $w'(y)=-\frac{1}{2}e^{-\frac{1}{2}y}\neq 0$ when $y>0$
                \begin{equation*}
                    \begin{split}
                        f(y)=&f(w(y))|w'(y)|\\
                            =&\frac{1}{2}e^{-\frac{1}{2}y}
                    \end{split}
                \end{equation*}
                and $f(y)=0$ elsewhere,
                which is a gamma distribution with parameters $\alpha=1$ and $\beta=2$
            }
        \subsection{}
            \paragraph{
                Let $w(y)=y^{-\gamma}$, then $w'(y)=-\gamma y^{-\gamma-1}\neq 0$ when $y>1$. Since $\gamma>0$
                \begin{equation*}
                    \begin{split}
                        g(y)=&f(w(y))|w'(y)|\\
                            =&\frac{\gamma}{y^{1+\gamma}}\\
                    \end{split}
                \end{equation*}
                when $y>1$, and $g(y)=0$ elsewhere.
            }
    \section{}
        \paragraph{
            \begin{equation*}
                \begin{split}
                    M_X(t)=&\mathbb{E}[e^{tX}]\\
                        =&\sum_{x=1}^\infty 2e^{tx}(\frac{1}{3})^x\\
                    \mu'_1=&\frac{d}{dt}M_X(t)|_{t=0}\\
                        =&\sum_{x=1}^\infty 2xe^{tx}(\frac{1}{3})^x|_{t=0}\\
                        =&\sum_{x=1}^\infty 2x(\frac{1}{3})^x\\
                    \mu'_2=&\frac{d^2}{dt^2}M_X(t)\\
                        =&\frac{d}{dt}\sum_{x=1}^\infty 2xe^{tx}(\frac{1}{3})^x|_{t=0}\\
                        =&\sum_{x=1}^\infty 2x^2e^{tx}(\frac{1}{3})^x|_{t=0}\\
                        =&\sum_{x=1}^\infty 2x^2(\frac{1}{3})^x\\
                \end{split}
            \end{equation*}
        }
    
    \section{}
        \paragraph{
            We know that
            $$f(x)=1$$ 
            when $0<x<1$
            , and $f(x)=0$ elsewhere.
            \begin{equation*}
                \begin{split}
                    M_X(t)=&\mathbb{E}[e^{tX}]\\
                        =&\int_0^1 e^{tx} 1 dx\\
                        =&\frac{e^t-1}{t}\\
                    \mu'_1=&\frac{d}{dt}M_X(t)|_{t=0}\\
                        =&\frac{e^t(t-1)+1}{t^2}|_{t=0}\\
                        =&\\
                    \mu'_2=&\frac{d^2}{dt^2}M_X(t)|_{t=0}\\    
                        =&\frac{d}{dt}\frac{e^t(t-1)+1}{t^2}|_{t=0}\\
                        =&\frac{e^tt^3-3e^tt+2e^t-2}{t^3}|_{t=0}\\
                        =&\\
                \end{split}
            \end{equation*}
        }
    
    \section{}
        \paragraph{
            \begin{equation*}
                \begin{split}
                    R_X(t)=&\log M_X(t)\\
                    R'_X(t)=&\frac{1}{M_X(t)}\frac{d}{dt}M_X(t)\\  
                    R'_X(0)=&\frac{1}{M_X(0)}\frac{d}{dt}M_X(t)|_{t=0}\\
                        =&\frac{d}{dt}M_X(t)|_{t=0}\\
                        =&\mu\\
                    R''_X(t)=&\frac{d}{dt}R'_X(t)\\   
                        =&\frac{M_X(t)\frac{d^2}{dt^2}M_X(t)-(\frac{d}{dt}M_X(t))^2}{M_X(t)^2}\\
                    R''_X(0)=&\frac{M_X(0)\frac{d^2}{dt^2}M_X(0)-(\frac{d}{dt}M_X(0))^2}{M_X(0)^2}\\
                        =&\mathbb{E}[X^2]-\mu^2\\
                        =&\sigma^2
                \end{split}
            \end{equation*}
            Let $$M_X(t)=e^{4(e^t-1)}$$
            then
            \begin{equation*}
                \begin{split}
                    R_X(t)=&\log M_X(t)\\  
                        =&4(e^t-1)\\
                    R'_X(t)=&4e^t\\
                    R'_X(0)=&4\\
                    R''_X(t)=&4e^t\\
                    R''_X(0)=&4\\
                \end{split}
            \end{equation*}
            Thus, the mean of a random variable $X$ is $\mu=4$ and the variance of $X$ is $\sigma^2=4$
        } 
    \section{}
        \paragraph{
            \begin{equation*}
                \begin{split}
                    M_X(t)=&\int_{-\infty}^{+\infty} e^{tx}f(x)dx\\
                        =&\int_{-\infty}^{+\infty} e^{tx}\frac{1}{2}e^{-|x|}dx\\
                        =&\int_{-\infty}^0 e^{tx}\frac{1}{2}e^{x}dx+\int_{0}^{+\infty} e^{tx}\frac{1}{2}e^{-x}dx\\
                        =&\frac{1}{2}[\frac{1}{t+1}e^{(t+1)x}|_{-\infty}^0+\frac{1}{t-1}e^{(t-1)x}|_0^{+\infty}]
                \end{split}
            \end{equation*}
            It is easy to know that when $t\leq-1$ or $t\geq 1$ , $M_X(t)$ is not definited. Thus,$$M_X(t)=\frac{1}{1-t^2}$$ when $t\in (-1,1)$
        }

    \section{}
        \paragraph{
            We get 
            $f(x)=\frac{3.3^x}{x!}e^{-3.3}$
        }
        \subsection{}   
            \paragraph{
               $$P(X=2)=f(2)=\frac{3.3^2}{2}e^{-3.3}\approx 0.2008$$
            }
        \subsection{}
            \paragraph{
                \begin{equation*}
                    \begin{split}
                        P=&P_2^2(f(0)f(5)+f(1)f(4)+f(2)f(3))\\
                            =&2\times e^{-3.3}\times(\frac{3.3^0}{0!}\frac{3.3^5}{5!}+\frac{3.3^1}{1!}\frac{3.3^4}{4!}+\frac{3.3^2}{2!}\frac{3.3^3}{3!})\\
                            =&3.3^5\times 2 \times e^{-3.3}\times(\frac{1}{0!}\frac{1}{5!}+\frac{1}{1!}\frac{1}{4!}+\frac{1}{2!}\frac{1}{3!})\\
                            \approx& 3.8491
                    \end{split}
                \end{equation*}
            }

    \section{}
        \paragraph{
            We get 
            $$f(x)=\frac{1}{5}e^{-\frac{x}{5}}$$
        }
        \subsection{}
            \paragraph{
                \begin{equation*}
                    \begin{split}
                        P=&\int_0^8\int_0^{8-x} \frac{1}{5}e^{-\frac{x}{5}}\frac{1}{5}e^{-\frac{y}{5}} dydx\\
                            =&\int_0^8\frac{1}{5}e^{-\frac{x}{5}}(-e^{-\frac{y}{5}})|_{y=0}^{8-x}dx\\
                            =&\int _0^8 \frac{1}{5}e^{-\frac{x}{5}}(1-e^{\frac{x-8}{5}})dx\\
                            =&\int_0^8\frac{1}{5}(e^{-\frac{x}{5}}-e^{-\frac{8}{5}})dx\\
                            =&(-e^{-\frac{x}{5}}-\frac{1}{5}e^{-\frac{8}{5}}x)|_{x=0}^8\\
                            =& 1-\frac{13}{5}e^{-\frac{8}{5}}\\
                            \approx&0.4751\\
                    \end{split}
                \end{equation*}
            }
        \subsection{}
            \paragraph{
                \begin{equation*}
                    \begin{split}
                        P=&\int _0^\infty \int _0 ^\infty \int_{12-x-y} ^\infty \frac{1}{125}e^{-\frac{1}{5}(x+y+z)}dzdydx\\
                            =&\int _0^\infty \int _0 ^\infty -\frac{1}{25}e^{-\frac{1}{5}(x+y)-\frac{1}{5}z}|_{z=12-x-y}^\infty dydx
                    \end{split}
                \end{equation*}
            }

    \section{}
        \paragraph{
            We get$$f(x)=\frac{1}{9}e^{-\frac{x}{9}}$$
        }
        \subsection{}
            \paragraph{
                \begin{equation*}
                    \begin{split}
                        P=&\int _0 ^{20} f(x)dx\\
                            =&\int _0 ^{20} \frac{1}{9}e^{-\frac{x}{9}}dx\\
                            =&-e^{-\frac{x}{9}}|_0^{20}\\
                            =&1-e^{-\frac{20}{9}}\\
                            \approx&0.8916
                    \end{split}
                \end{equation*}
            }
        \subsection{}
            \paragraph{
                \begin{equation*}
                    \begin{split}
                        P=&\int_0^{20}\int_{0}^{20-x}\frac{1}{81}e^{-\frac{1}{9}(x+y)}dydx\\
                            =&\int_0^{20}-\frac{1}{9}e^{-\frac{1}{9}(x+y)}|_0^{20-x}dx\\
                            =&\int_0^{20}\frac{1}{9}(e^{-\frac{1}{9}x}-e^{-\frac{20}{9}})dx\\
                            =&-e^{-\frac{1}{9}x}-\frac{1}{9}e^{-\frac{20}{9}}x|_0^{20}\\
                            =&1-\frac{29}{9}e^{-\frac{20}{9}}\\
                            \approx&0.6508
                    \end{split}
                \end{equation*}
            }
                
\end{document}