\documentclass{article}
\usepackage{setspace}
\usepackage{amsmath}
\usepackage{amssymb}
\usepackage{amsthm}
\usepackage{graphicx} 
\usepackage{float} 
\usepackage{fancyhdr}                                
\usepackage{lastpage}                                           
\usepackage{layout}   
\usepackage{subfigure} 
\pagestyle{fancy}  
\lhead{ZHANG HUAKANG}
\chead{Assignment 5} 
\rhead{DB92760} 
\renewcommand{\baselinestretch}{1.05}
\title{Assignment 4 of MATH 2005}
\author{ZHANG Huakang/DB92760}

\begin{document}
    \maketitle
    \section{}
    \paragraph{
        \begin{equation*}
            \begin{split}
                E[X]=&\sum_{n=1} ^knf(n)\\
                    =&\frac{1}{k}\sum_{n=1}^k n\\
                    =&\frac{1}{k}\ \frac{k(k+1)}{2}\\
                    =&\frac{k+1}{2}\\
                var(X)=&\sum_{n=1}^k (n-E[X])^2f(n)\\
                    =&\frac{1}{k}\sum_{n=1}^k(n-\frac{k+1}{2})^2\\
                    =&\frac{1}{k}\sum_{n=1}^k(n^2-n(k+1)-\frac{(k+1)^2}{4})\\
                    =&\frac{1}{k}(\frac{k(k+1)(2k+1)}{6}-\frac{k(k+1)}{2}(k+1)+\frac{k(k+1)^2}{4})\\
                    =&\frac{(k+1)(2k+1)}{6}-\frac{(k+1)^2}{2}+\frac{(k+1)^2}{4}\\
                    =&\frac{(k+1)(2k+1)}{6}-\frac{(k+1)^2}{4}\\
                    =&(k+1)\frac{k-1}{12}\\
                    =&\frac{k^2-1}{12}
            \end{split}
        \end{equation*}
    }

    \section{}
    \paragraph{
        \begin{equation*}
            \begin{split}
                b(x;n,\theta)=&C_n^x\theta^x(1-\theta)^{n-x}\\
                    =& C_{n}^{n-x}(1-\theta)^{n-x}\theta^x\\
                    =&b(n-x;n,1-\theta)\\
            \end{split}
        \end{equation*}
    }
    \subsection{}
        \paragraph{
            \begin{equation*}
                \begin{split}
                    B(n-x;n,1-\theta)-B(n-x-1;n,1-\theta)=&\sum_{y=0}^{n-x}b(y;n,1-\theta)\\
                        &-\sum_{y=0}^{n-x-1}b(y;n,1-\theta)\\
                        =&b(n-x;n,1-\theta)\\
                        =&b(x;n,\theta)
                \end{split}
            \end{equation*}
        }
    \subsection{}
        \paragraph{
            $$B(n;n,1-\theta)=\sum_{y=0}^nb(y;n,\theta)=1$$
            \begin{equation*}
                \begin{split}
                    B(x;n,\theta)=&\sum_{y=0}^xb(y;n,\theta)\\
                        =&\sum_{y=0}^x[B(n-y;n,1-\theta)-B(n-y-1;n,1-\theta)]\\
                        =&B(n;n,1-\theta)-B(n-x-1;n,1-\theta)\\
                        =&1-B(n-x-1;n,1-\theta)\\
                \end{split}
            \end{equation*}
        }

\end{document}