\documentclass{article}
\usepackage{setspace}
\usepackage{amsmath}
\usepackage{amstext}
\usepackage{amssymb}
\usepackage{amsthm}
\usepackage{graphicx} 
\usepackage{float} 
\usepackage{fancyhdr}                                
\usepackage{lastpage}          
\usepackage{textcomp}                               
\usepackage{layout}   
\usepackage{subfigure} 
\pagestyle{fancy}  
\lhead{ZHANG HUAKANG}
\chead{Assignment 6} 
\rhead{DB92760} 
\renewcommand{\baselinestretch}{1.05}
\title{Assignment 6 of MATH 2005}
\author{ZHANG Huakang/DB92760}

\begin{document}
    \maketitle
    \section{}
        \begin{equation*}
            \begin{split}
                \mathbb{P}[X< -\theta\log(1-p)]=&\int_{-\infty}^{-\theta\log(1-p)}f(y)dy\\
                    =&\int_0^{-\theta\log(1-p)}\frac{1}{\theta}e^{-\frac{y}{\theta}}dy\\
                    =&-e^{-\frac{y}{\theta}}|_{0}^{-\theta\log(1-p)}\\
                    =&1-(1-p)\\
                    =&p
            \end{split}
        \end{equation*}

    \section{}
        \begin{equation*}
            \begin{split}
                \mathbb{E}[X]=&\int_{-\infty}^{\infty}xf(x)dx\\
                    =&\int_{0}^{\infty}x2\alpha xe^{-\alpha x^2}dx\\
                    =&2\alpha\int_{0}^{\infty} x^2e^{-\alpha x^2}dx\\
            \end{split}
        \end{equation*}
        Let $u=x$ and $v'=xe^{-\alpha x^2}$, thus $u'=1$ and $v=-\frac{1}{2\alpha}e^{-\alpha x^2}$
        \begin{equation*}
            \begin{split}
                \int x^2e^{-\alpha x^2}dx=&-\frac{x}{2\alpha}e^{-\alpha x^2}+\int \frac{1}{2\alpha}e^{-\alpha x^2}dx\\
                    =&-\frac{x}{2\alpha}e^{-\alpha x^2}+\frac{\sqrt{\pi}erf(\sqrt{\alpha}x)}{2\sqrt{\alpha}}\\
            \end{split}
        \end{equation*}
        Thus
        \begin{equation*}
            \begin{split}
                \mathbb{E}[X]=&[-\frac{x}{2\alpha}e^{-\alpha x^2}+\frac{\sqrt{\pi}erf(\sqrt{\alpha}x)}{2\sqrt{\alpha}}]|_0^{\infty}\\
                    =&\frac{\sqrt{\pi}}{2\sqrt{\alpha}}
            \end{split}
        \end{equation*}
        And 
        \begin{equation*}
            \begin{split}
                \mathbb{E}[X^2]=&\int_{-\infty}^{\infty}x^2f(x)dx\\
                    =&\int_{0}^{\infty}x^22\alpha xe^{-\alpha x^2}dx\\
                    =&2\alpha\int_{0}^{\infty}x^3e^{-\alpha x^2}dx\\
            \end{split}
        \end{equation*}
        Let $u=x^2$ and $v'=xe^{\alpha x^2}$, thus $u'=2x$ and $v=-\frac{1}{2\alpha}e^{-\alpha x^2}$
        \begin{equation*}
            \begin{split}
                \int x^3e^{-\alpha x^2}dx=&-\frac{x^2}{2\alpha}e^{-\alpha x^2}+\int \frac{x}{\alpha}e^{-\alpha x^2}
            \end{split}
        \end{equation*}

\end{document}